rupicola/refinements2/Examples.fst
@@ -1,0 +1,44 @@
+module Examples
+
+let test_just_true
+  : bool -> (x:bool{x == true})
+  = fun x -> true
+
+assume val some_ref : Type0
+let test_moving_ref
+  : _:bool{some_ref} -> _:unit{some_ref}
+  = fun _ -> ()
+
+let test_always_false
+  : bool -> y:bool{y == false}
+  = fun x -> if x then false else x
+
+let test_always_false_complex
+  : bool -> y:bool{y == false}
+  = fun x -> if x then if x then false else true else false
+
+let test_if_x
+  : (f:(x:bool{x == true}) -> bool) -> bool -> bool
+  = fun f x -> if x then f x else false
+
+assume val p_ref : bool -> Type0
+assume val q_ref : bool -> Type0
+let test_p_implies_q
+  : (f: (x:bool{p_ref x} -> _:unit{q_ref x})) -> (x:bool{p_ref x}) -> (x:bool{q_ref x})
+  = fun f x -> f x; x
+
+let test_false_elim0
+  : bool -> bool
+  = fun x -> if x then if x then true else false_elim () else true
+
+let test_false_elim1
+  : x:unit{False} -> Tot bool
+  = fun x -> false_elim ()
+
+let test_false_elim2
+  : f:(unit -> x:bool{x == true}) -> Tot bool
+  = fun f -> if f () then true else false_elim ()
+
+let test_erase_ref
+  : (x:bool{x == true} -> bool)
+  = fun x -> x
